@prefix : <http://www.semanticweb.org/owl/owlapi/turtle#> .
@prefix owl: <http://www.w3.org/2002/07/owl#> .
@prefix rdf: <http://www.w3.org/1999/02/22-rdf-syntax-ns#> .
@prefix xml: <http://www.w3.org/XML/1998/namespace> .
@prefix xsd: <http://www.w3.org/2001/XMLSchema#> .
@prefix rdfs: <http://www.w3.org/2000/01/rdf-schema#> .
@prefix LoSeOn: <https://github.com/Michael-Gloeckner/LoSeOn#> .
@base <https://github.com/Michael-Gloeckner/LoSeOn> .

<https://github.com/Michael-Gloeckner/LoSeOn> rdf:type owl:Ontology ;
                                              
                                              rdfs:label "LoSeOn"@en ;
                                              
                                              rdfs:comment "This is an ontology design pattern for logistics services."@en .


#################################################################
#
#    Object Properties
#
#################################################################


###  https://github.com/Michael-Gloeckner/LoSeOn#IsConnectedBy

LoSeOn:IsConnectedBy rdf:type owl:ObjectProperty ;
                     
                     rdfs:label "IsConnectedBy"@en ;
                     
                     rdfs:comment "describes the connection of something by something"@en ;
                     
                     rdfs:range LoSeOn:Flow ;
                     
                     rdfs:domain LoSeOn:LogisticsService .



###  https://github.com/Michael-Gloeckner/LoSeOn#IsConsumedBy

LoSeOn:IsConsumedBy rdf:type owl:ObjectProperty ;
                    
                    rdfs:label "IsConsumedBy"@en ;
                    
                    rdfs:comment "describes the consumption of something by something"@en ;
                    
                    owl:inverseOf LoSeOn:IsProvidedBy ;
                    
                    rdfs:domain LoSeOn:LogisticsService ;
                    
                    rdfs:range LoSeOn:LogisticsService ,
                               LoSeOn:LogisticsStakeholder ;
                    
                    rdfs:domain LoSeOn:Resource .



###  https://github.com/Michael-Gloeckner/LoSeOn#IsContrainedBy

LoSeOn:IsContrainedBy rdf:type owl:ObjectProperty ;
                      
                      rdfs:label "IsContrainedBy"@en ;
                      
                      rdfs:comment "describes constrain of something by something"@en ;
                      
                      rdfs:range LoSeOn:Contraints ;
                      
                      rdfs:domain LoSeOn:LogisticsService .



###  https://github.com/Michael-Gloeckner/LoSeOn#IsEnabledBy

LoSeOn:IsEnabledBy rdf:type owl:ObjectProperty ;
                   
                   rdfs:label "IsEnabledBy"@en ;
                   
                   rdfs:comment "describes the enabling of sommething by sommething"@en ;
                   
                   rdfs:domain LoSeOn:Flow ;
                   
                   rdfs:range LoSeOn:Resource ;
                   
                   rdfs:domain LoSeOn:Transformation .



###  https://github.com/Michael-Gloeckner/LoSeOn#IsMeasuredBy

LoSeOn:IsMeasuredBy rdf:type owl:ObjectProperty ;
                    
                    rdfs:label "IsMeasuredBy"@en ;
                    
                    rdfs:comment "describes measurement of something by something"@en ;
                    
                    rdfs:domain LoSeOn:LogisticsService ;
                    
                    rdfs:range LoSeOn:SLA .



###  https://github.com/Michael-Gloeckner/LoSeOn#IsPerformedBy

LoSeOn:IsPerformedBy rdf:type owl:ObjectProperty ;
                     
                     rdfs:label "IsPerformedBy"@en ;
                     
                     rdfs:comment "describes the performance of something by something"@en ;
                     
                     rdfs:range LoSeOn:Active ,
                                LoSeOn:LogisticsService ;
                     
                     rdfs:domain LoSeOn:Transformation .



###  https://github.com/Michael-Gloeckner/LoSeOn#IsProvidedBy

LoSeOn:IsProvidedBy rdf:type owl:ObjectProperty ;
                    
                    rdfs:label "IsProvidedBy"@en ;
                    
                    rdfs:comment "describes the provision of something by something"@en ;
                    
                    rdfs:domain LoSeOn:LogisticsService ;
                    
                    rdfs:range LoSeOn:LogisticsStakeholder .





#################################################################
#
#    Classes
#
#################################################################


###  https://github.com/Michael-Gloeckner/LoSeOn#Active

LoSeOn:Active rdf:type owl:Class ;
              
              rdfs:label "Active"@en ;
              
              rdfs:subClassOf LoSeOn:Power ;
              
              rdfs:comment "An Active Resource posseses the ability of transforming a logistics entity by itself."@en .



###  https://github.com/Michael-Gloeckner/LoSeOn#Character

LoSeOn:Character rdf:type owl:Class ;
                 
                 rdfs:label "Character"@en ;
                 
                 rdfs:subClassOf LoSeOn:Resource ;
                 
                 rdfs:comment "The Character describes the consistence of a Resource. It is either Informational OR Physical."@en .



###  https://github.com/Michael-Gloeckner/LoSeOn#Contraints

LoSeOn:Contraints rdf:type owl:Class ;
                  
                  rdfs:label "Constraints"@en ;
                  
                  rdfs:comment "Contraints define external requirements that have to be fulfilled by a logistics service. They are either of mandatory (such as official laws) or non-mandatory nature (such as customer requirements)."@en .



###  https://github.com/Michael-Gloeckner/LoSeOn#Control

LoSeOn:Control rdf:type owl:Class ;
               
               rdfs:label "Control"@en ;
               
               rdfs:subClassOf LoSeOn:Flow ;
               
               rdfs:comment "Control is the Flow of information in order to trigger following LogisticsService."@en .



###  https://github.com/Michael-Gloeckner/LoSeOn#Cost

LoSeOn:Cost rdf:type owl:Class ;
            
            rdfs:label "Cost"@en ;
            
            rdfs:subClassOf LoSeOn:Transformation ;
            
            rdfs:comment "A LogisticsService tranforms costs of the overall service in a certain kind of way. Usually Costs increase by the usage of a Service."@en .



###  https://github.com/Michael-Gloeckner/LoSeOn#Economic

LoSeOn:Economic rdf:type owl:Class ;
                
                rdfs:label "Economic"@en ;
                
                rdfs:subClassOf LoSeOn:NonMandatory ;
                
                rdfs:comment "Economic contraints aim at delivering complex logistics services in a cheap way."@en .



###  https://github.com/Michael-Gloeckner/LoSeOn#Environmental

LoSeOn:Environmental rdf:type owl:Class ;
                     
                     rdfs:label "Environmental"@en ;
                     
                     rdfs:subClassOf LoSeOn:NonMandatory ;
                     
                     rdfs:comment "Environmental constraints aim at delivering complex logistics services in a einvironmentally friendly way, e.g. with a reduced carbon footprint."@en .



###  https://github.com/Michael-Gloeckner/LoSeOn#Flow

LoSeOn:Flow rdf:type owl:Class ;
            
            rdfs:label "Flow"@en ;
            
            rdfs:comment "The several flows connect two or more logistics services with each other. Different kinds of flows can be distinguished."@en .



###  https://github.com/Michael-Gloeckner/LoSeOn#Information

LoSeOn:Information rdf:type owl:Class ;
                   
                   rdfs:label "Information"@en ;
                   
                   rdfs:subClassOf LoSeOn:Transformation ;
                   
                   rdfs:comment "A LogisticsService could transform Information in a certain kind of way."@en .



###  https://github.com/Michael-Gloeckner/LoSeOn#Informational

LoSeOn:Informational rdf:type owl:Class ;
                     
                     rdfs:label "Informational"@en ;
                     
                     rdfs:subClassOf LoSeOn:Character ,
                                     LoSeOn:Flow ;
                     
                     rdfs:comment "Either one of the Flows connecting LogisticsService or the characteristics of a certain Resource could be Informational."@en .



###  https://github.com/Michael-Gloeckner/LoSeOn#Location

LoSeOn:Location rdf:type owl:Class ;
                
                rdfs:label "Location"@en ;
                
                rdfs:subClassOf LoSeOn:Transformation ;
                
                rdfs:comment "A LogisticsService could transform Location in a certain kind of way."@en .



###  https://github.com/Michael-Gloeckner/LoSeOn#LogisticsService

LoSeOn:LogisticsService rdf:type owl:Class ;
                        
                        rdfs:label "LogisticsService"@en ;
                        
                        rdfs:comment """A Logistics Service is characterized by general service characteristics. This includes a pre-defined set of inputs, outputs and transformations that take place during its execution. Further important is the usage of resources and the application of knowledge and skills within activities or processes in order to generate benefit for another entity or for the entity itself.

A Logistics Service is a Service conducted within the logistics domain and logistics purpose."""@en .



###  https://github.com/Michael-Gloeckner/LoSeOn#LogisticsStakeholder

LoSeOn:LogisticsStakeholder rdf:type owl:Class ;
                            
                            rdfs:label "LogisticsStakeholder"@en ;
                            
                            rdfs:comment "A LogisticsStakeholder is a natural or a legal person involved in the planning, operation or monitoring of a LogisticsService. It either provides, uses or manages the service or is in another way connected to it."@en .



###  https://github.com/Michael-Gloeckner/LoSeOn#Mandatory

LoSeOn:Mandatory rdf:type owl:Class ;
                 
                 rdfs:label "Mandatory"@en ;
                 
                 rdfs:subClassOf LoSeOn:Contraints ;
                 
                 owl:disjointWith LoSeOn:NonMandatory ;
                 
                 rdfs:comment "Mandatory contraints are requirements by official, public or governmental institutions."@en .



###  https://github.com/Michael-Gloeckner/LoSeOn#NonMandatory

LoSeOn:NonMandatory rdf:type owl:Class ;
                    
                    rdfs:label "NonMandatory"@en ;
                    
                    rdfs:subClassOf LoSeOn:Contraints ;
                    
                    rdfs:comment "Non-mandatory contraints are requirements by customers. They are not obligatory like the mandatory contraints from legal institutions."@en .



###  https://github.com/Michael-Gloeckner/LoSeOn#Passive

LoSeOn:Passive rdf:type owl:Class ;
               
               rdfs:label "Passive"@en ;
               
               rdfs:subClassOf LoSeOn:Power ;
               
               rdfs:comment "An Passive Resource does not posses the ability of transforming a logistics entity by itself. It is transformed by an Active Resource."@en .



###  https://github.com/Michael-Gloeckner/LoSeOn#Physical

LoSeOn:Physical rdf:type owl:Class ;
                
                rdfs:label "Physical"@en ;
                
                rdfs:subClassOf LoSeOn:Character ,
                                LoSeOn:Flow ;
                
                rdfs:comment "Either one of the Flows connecting LogisticsService or the characteristics of a certain Resource could be Physical."@en .



###  https://github.com/Michael-Gloeckner/LoSeOn#Power

LoSeOn:Power rdf:type owl:Class ;
             
             rdfs:label "Power"@en ;
             
             rdfs:subClassOf LoSeOn:Resource ;
             
             rdfs:comment "The Power describes the ability of a Resource. It is either Active OR Passive."@en .



###  https://github.com/Michael-Gloeckner/LoSeOn#Product

LoSeOn:Product rdf:type owl:Class ;
               
               rdfs:label "Product"@en ;
               
               rdfs:subClassOf LoSeOn:Transformation ;
               
               rdfs:comment "A LogisticsService could transform Product in a certain kind of way."@en .



###  https://github.com/Michael-Gloeckner/LoSeOn#Quality

LoSeOn:Quality rdf:type owl:Class ;
               
               rdfs:label "Quality"@en ;
               
               rdfs:subClassOf LoSeOn:Transformation ;
               
               rdfs:comment "A LogisticsService could transform Quality of a Product in a certain kind of way."@en .



###  https://github.com/Michael-Gloeckner/LoSeOn#Quantity

LoSeOn:Quantity rdf:type owl:Class ;
                
                rdfs:label "Quantity"@en ;
                
                rdfs:subClassOf LoSeOn:Transformation ;
                
                rdfs:comment "A LogisticsService could transform Quantity of a Product in a certain kind of way."@en .



###  https://github.com/Michael-Gloeckner/LoSeOn#Resource

LoSeOn:Resource rdf:type owl:Class ;
                
                rdfs:label "Resource"@en ;
                
                rdfs:comment "A Resource is consumed during the conduction of a LogisticsService. It is either available again afterward (such as warehouse capacity or a truck) or not (such as some kind of one-way packaging)."@en .



###  https://github.com/Michael-Gloeckner/LoSeOn#SLA

LoSeOn:SLA rdf:type owl:Class ;
           
           rdfs:label "ServiceLevelAgreements"@en ;
           
           rdfs:comment "ServiceLevelAgreements determine the quality of the service, e.g. lead time, accuracy."@en .



###  https://github.com/Michael-Gloeckner/LoSeOn#Social

LoSeOn:Social rdf:type owl:Class ;
              
              rdfs:label "Social"@en ;
              
              rdfs:subClassOf LoSeOn:NonMandatory ;
              
              rdfs:comment "Social contraints aim at delivering complex logistics services in a socially reasonable way, e.g. with a guaranteed minimum wage."@en .



###  https://github.com/Michael-Gloeckner/LoSeOn#Time

LoSeOn:Time rdf:type owl:Class ;
            
            rdfs:label "Time"@en ;
            
            rdfs:subClassOf LoSeOn:Transformation ;
            
            rdfs:comment "Time describes the temporal starting and ending points of a LogisticsService."@en ;
            
            rdfs:seeAlso "http://www.ontologydesignpatterns.org/cp/owl/timeinterval.owl"@en .



###  https://github.com/Michael-Gloeckner/LoSeOn#Transformation

LoSeOn:Transformation rdf:type owl:Class ;
                      
                      rdfs:label "Transformation"@en ;
                      
                      rdfs:comment "Transformation contains the possible dimensions that could be changed during a LogisticsService."@en .



[ rdfs:label "LoSeOn"^^xsd:string
] .

###  Generated by the OWL API (version 3.4.2) http://owlapi.sourceforge.net

